enforce that registers only contain 64 bits when calling

theories/calling_convention.v
@@ -6,32 +6,59 @@ Require Import isla.sys_regs.
 Definition tmp_registers : list string :=
   ["R9"; "R10"; "R11"; "R12"; "R13"; "R14"; "R15"; "R16"; "R17"].
 
-Definition c_call `{!islaG Σ} `{!threadG} (stack_size : Z) (P : list valu → bv 64 → ((list valu → iProp Σ) → iProp Σ) → iProp Σ) : iProp Σ :=
+Definition c_call_ret `{!islaG Σ} `{!threadG} (stack_size : Z) (regs : list valu) (ret sp : bv 64) (Q : (list (bv 64) → iProp Σ)) : iProp Σ :=
+  reg_col sys_regs ∗
+  reg_col CNVZ_regs ∗
+  reg_col ((λ r, (KindReg r, BitsShape 64)) <$> ["R0"; "R1"; "R2"; "R3"; "R4"; "R5"; "R6"; "R7"]) ∗
+  reg_col ((λ r, (KindReg r, BitsShape 64)) <$> tmp_registers) ∗
+  reg_col (zip_with (λ r v, (KindReg r, ExactShape v)) ["R19"; "R20"; "R21"; "R22"; "R23"; "R24"; "R25"; "R26"; "R27"; "R28"; "R29"] regs) ∗
+  "R0" ↦ᵣ: λ r0, ∃ b0 : bv 64, ⌜r0 = RVal_Bits b0⌝ ∗
+  "R1" ↦ᵣ: λ r1, ∃ b1 : bv 64, ⌜r1 = RVal_Bits b1⌝ ∗
+  "R2" ↦ᵣ: λ r2, ∃ b2 : bv 64, ⌜r2 = RVal_Bits b2⌝ ∗
+  "R3" ↦ᵣ: λ r3, ∃ b3 : bv 64, ⌜r3 = RVal_Bits b3⌝ ∗
+  "R4" ↦ᵣ: λ r4, ∃ b4 : bv 64, ⌜r4 = RVal_Bits b4⌝ ∗
+  "R5" ↦ᵣ: λ r5, ∃ b5 : bv 64, ⌜r5 = RVal_Bits b5⌝ ∗
+  "R6" ↦ᵣ: λ r6, ∃ b6 : bv 64, ⌜r6 = RVal_Bits b6⌝ ∗
+  "R7" ↦ᵣ: λ r7, ∃ b7 : bv 64, ⌜r7 = RVal_Bits b7⌝ ∗
+  "R8" ↦ᵣ: λ r8, ∃ b8 : bv 64, ⌜r8 = RVal_Bits b8⌝ ∗
+  "R30" ↦ᵣ RVal_Bits ret ∗
+  "SP_EL2" ↦ᵣ RVal_Bits sp ∗
+  bv_sub_Z sp stack_size ↦ₘ? stack_size ∗
+  Q [b0; b1; b2; b3; b4; b5; b6; b7; b8].
+Global Instance : LithiumUnfold (@c_call_ret) := I.
+
+
+Definition c_call `{!islaG Σ} `{!threadG} (stack_size : Z) (P : list (bv 64) → bv 64 → ((list (bv 64) → iProp Σ) → iProp Σ) → iProp Σ) : iProp Σ :=
   ∃ (sp ret : bv 64),
   reg_col sys_regs ∗
   reg_col CNVZ_regs ∗
-  reg_col ((λ r, (KeyReg r, None)) <$> tmp_registers) ∗
-  "R0" ↦ᵣ: λ r0, "R1" ↦ᵣ: λ r1, "R2" ↦ᵣ: λ r2, "R3" ↦ᵣ: λ r3, "R4" ↦ᵣ: λ r4, "R5" ↦ᵣ: λ r5,
-  "R6" ↦ᵣ: λ r6, "R7" ↦ᵣ: λ r7, "R8" ↦ᵣ: λ r8, "R19" ↦ᵣ: λ r19, "R20" ↦ᵣ: λ r20, "R21" ↦ᵣ: λ r21,
-  "R22" ↦ᵣ: λ r22, "R23" ↦ᵣ: λ r23, "R24" ↦ᵣ: λ r24, "R25" ↦ᵣ: λ r25, "R26" ↦ᵣ: λ r26, "R27" ↦ᵣ: λ r27,
-  "R28" ↦ᵣ: λ r28, "R29" ↦ᵣ: λ r29,
+  reg_col ((λ r, (KindReg r, BitsShape 64)) <$> tmp_registers) ∗
+  "R0" ↦ᵣ: λ r0, ∃ b0 : bv 64, ⌜r0 = RVal_Bits b0⌝ ∗
+  "R1" ↦ᵣ: λ r1, ∃ b1 : bv 64, ⌜r1 = RVal_Bits b1⌝ ∗
+  "R2" ↦ᵣ: λ r2, ∃ b2 : bv 64, ⌜r2 = RVal_Bits b2⌝ ∗
+  "R3" ↦ᵣ: λ r3, ∃ b3 : bv 64, ⌜r3 = RVal_Bits b3⌝ ∗
+  "R4" ↦ᵣ: λ r4, ∃ b4 : bv 64, ⌜r4 = RVal_Bits b4⌝ ∗
+  "R5" ↦ᵣ: λ r5, ∃ b5 : bv 64, ⌜r5 = RVal_Bits b5⌝ ∗
+  "R6" ↦ᵣ: λ r6, ∃ b6 : bv 64, ⌜r6 = RVal_Bits b6⌝ ∗
+  "R7" ↦ᵣ: λ r7, ∃ b7 : bv 64, ⌜r7 = RVal_Bits b7⌝ ∗
+  "R8" ↦ᵣ: λ r8, ⌜valu_has_shape r8 (BitsShape 64)⌝ ∗
+  "R19" ↦ᵣ: λ r19, ⌜valu_has_shape r19 (BitsShape 64)⌝ ∗
+  "R20" ↦ᵣ: λ r20, ⌜valu_has_shape r20 (BitsShape 64)⌝ ∗
+  "R21" ↦ᵣ: λ r21, ⌜valu_has_shape r21 (BitsShape 64)⌝ ∗
+  "R22" ↦ᵣ: λ r22, ⌜valu_has_shape r22 (BitsShape 64)⌝ ∗
+  "R23" ↦ᵣ: λ r23, ⌜valu_has_shape r23 (BitsShape 64)⌝ ∗
+  "R24" ↦ᵣ: λ r24, ⌜valu_has_shape r24 (BitsShape 64)⌝ ∗
+  "R25" ↦ᵣ: λ r25, ⌜valu_has_shape r25 (BitsShape 64)⌝ ∗
+  "R26" ↦ᵣ: λ r26, ⌜valu_has_shape r26 (BitsShape 64)⌝ ∗
+  "R27" ↦ᵣ: λ r27, ⌜valu_has_shape r27 (BitsShape 64)⌝ ∗
+  "R28" ↦ᵣ: λ r28, ⌜valu_has_shape r28 (BitsShape 64)⌝ ∗
+  "R29" ↦ᵣ: λ r29, ⌜valu_has_shape r29 (BitsShape 64)⌝ ∗
   "R30" ↦ᵣ RVal_Bits ret ∗
   "SP_EL2" ↦ᵣ RVal_Bits sp ∗
   ⌜stack_size < bv_unsigned sp < 2 ^ 52⌝ ∗
   bv_sub_Z sp stack_size ↦ₘ? stack_size ∗
-  P [r0; r1; r2; r3; r4; r5; r6; r7] sp (λ Q,
+  P [b0; b1; b2; b3; b4; b5; b6; b7] sp (λ Q,
   instr_pre (bv_unsigned ret) (
-      reg_col sys_regs ∗
-      reg_col CNVZ_regs ∗
-      reg_col ((λ r, (KeyReg r, None)) <$> ["R0"; "R1"; "R2"; "R3"; "R4"; "R5"; "R6"; "R7"]) ∗
-      reg_col ((λ r, (KeyReg r, None)) <$> tmp_registers) ∗
-      "R0" ↦ᵣ: λ r0', "R1" ↦ᵣ: λ r1', "R2" ↦ᵣ: λ r2', "R3" ↦ᵣ: λ r3', "R4" ↦ᵣ: λ r4',
-      "R5" ↦ᵣ: λ r5', "R6" ↦ᵣ: λ r6', "R7" ↦ᵣ: λ r7', "R8" ↦ᵣ: λ r8',
-      "R19" ↦ᵣ r19 ∗ "R20" ↦ᵣ r20 ∗ "R21" ↦ᵣ r21 ∗ "R22" ↦ᵣ r22 ∗ "R23" ↦ᵣ r23 ∗ "R24" ↦ᵣ r24 ∗
-      "R25" ↦ᵣ r25 ∗ "R26" ↦ᵣ r26 ∗ "R27" ↦ᵣ r27 ∗ "R28" ↦ᵣ r28 ∗ "R29" ↦ᵣ r29 ∗
-      "R30" ↦ᵣ RVal_Bits ret ∗
-      "SP_EL2" ↦ᵣ RVal_Bits sp ∗
-      bv_sub_Z sp stack_size ↦ₘ? stack_size ∗
-      Q [r0'; r1'; r2'; r3'; r4'; r5'; r6'; r7'; r8']
+      c_call_ret stack_size [r19; r20; r21; r22; r23; r24; r25; r26; r27; r28; r29] ret sp Q
   )).
 Global Instance : LithiumUnfold (@c_call) := I.
