theories/sys_regs.v
@@ -1,43 +1,32 @@
 Require Import isla.base.
 Require Import isla.automation.
 
-Definition sys_regs : list (reg_col_key * option valu) := [
-  (KeyReg "SCTLR_EL2" , Some (RVal_Bits [BV{64} 0x0000000004000002] ));
-  (KeyReg "SCR_EL3" , Some (RVal_Bits [BV{32} 0] ));
-  (KeyReg "TCR_EL2" , Some (RVal_Bits [BV{64} 0] ));
-  (KeyReg "CFG_ID_AA64PFR0_EL1_EL0" , Some (RVal_Bits [BV{4} 1] ));
-  (KeyReg "CFG_ID_AA64PFR0_EL1_EL1" , Some (RVal_Bits [BV{4} 1] ));
-  (KeyReg "CFG_ID_AA64PFR0_EL1_EL2" , Some (RVal_Bits [BV{4} 1] ));
-  (KeyReg "CFG_ID_AA64PFR0_EL1_EL3" , Some (RVal_Bits [BV{4} 1] ));
-  (KeyReg "OSLSR_EL1" , Some (RVal_Bits [BV{32} 0] ));
-  (KeyReg "OSDLR_EL1" , Some (RVal_Bits [BV{32} 0] ));
-  (KeyReg "EDSCR" , Some (RVal_Bits [BV{32} 0] ));
-  (KeyReg "MPIDR_EL1" , Some (RVal_Bits [BV{64} 0] ));
-  (KeyField "PSTATE" "SP" , Some (RVal_Bits [BV{1} 1] ));
-  (KeyField "PSTATE" "EL" , Some (RVal_Bits [BV{2} 2] ));
-  (KeyField "PSTATE" "nRW" , Some (RVal_Bits [BV{1} 0] ));
-  (KeyField "PSTATE" "D" , Some (RVal_Bits [BV{1} 1]))
+Definition sys_regs : list (reg_kind * valu_shape) := [
+  (KindReg "SCTLR_EL2" , ExactShape (RVal_Bits [BV{64} 0x0000000004000002] ));
+  (KindReg "SCR_EL3" , ExactShape (RVal_Bits [BV{32} 0] ));
+  (KindReg "TCR_EL2" , ExactShape (RVal_Bits [BV{64} 0] ));
+  (KindReg "CFG_ID_AA64PFR0_EL1_EL0" , ExactShape (RVal_Bits [BV{4} 1] ));
+  (KindReg "CFG_ID_AA64PFR0_EL1_EL1" , ExactShape (RVal_Bits [BV{4} 1] ));
+  (KindReg "CFG_ID_AA64PFR0_EL1_EL2" , ExactShape (RVal_Bits [BV{4} 1] ));
+  (KindReg "CFG_ID_AA64PFR0_EL1_EL3" , ExactShape (RVal_Bits [BV{4} 1] ));
+  (KindReg "OSLSR_EL1" , ExactShape (RVal_Bits [BV{32} 0] ));
+  (KindReg "OSDLR_EL1" , ExactShape (RVal_Bits [BV{32} 0] ));
+  (KindReg "EDSCR" , ExactShape (RVal_Bits [BV{32} 0] ));
+  (KindReg "MPIDR_EL1" , ExactShape (RVal_Bits [BV{64} 0] ));
+  (KindField "PSTATE" "SP" , ExactShape (RVal_Bits [BV{1} 1] ));
+  (KindField "PSTATE" "EL" , ExactShape (RVal_Bits [BV{2} 2] ));
+  (KindField "PSTATE" "nRW" , ExactShape (RVal_Bits [BV{1} 0] ));
+  (KindField "PSTATE" "D" , ExactShape (RVal_Bits [BV{1} 1]))
 ].
 
-Definition CNVZ_regs : list (reg_col_key * option valu) := [
-  (KeyField "PSTATE" "C", None);
-  (KeyField "PSTATE" "N", None);
-  (KeyField "PSTATE" "V", None);
-  (KeyField "PSTATE" "Z", None)
+Definition CNVZ_regs : list (reg_kind * valu_shape) := [
+  (KindField "PSTATE" "C", BitsShape 1);
+  (KindField "PSTATE" "N", BitsShape 1);
+  (KindField "PSTATE" "V", BitsShape 1);
+  (KindField "PSTATE" "Z", BitsShape 1)
 ].
 
 Definition sys_regs_map : reg_map :=
-  <[ "SCTLR_EL2" := RVal_Bits [BV{64} 0x0000000004000002] ]> $
-  <[ "SCR_EL3" := RVal_Bits [BV{32} 0] ]> $
-  <[ "TCR_EL2" := RVal_Bits [BV{64} 0] ]> $
-  <[ "CFG_ID_AA64PFR0_EL1_EL0" := RVal_Bits [BV{4} 1] ]> $
-  <[ "CFG_ID_AA64PFR0_EL1_EL1" := RVal_Bits [BV{4} 1] ]> $
-  <[ "CFG_ID_AA64PFR0_EL1_EL2" := RVal_Bits [BV{4} 1] ]> $
-  <[ "CFG_ID_AA64PFR0_EL1_EL3" := RVal_Bits [BV{4} 1] ]> $
-  <[ "OSLSR_EL1" := RVal_Bits [BV{32} 0] ]> $
-  <[ "OSDLR_EL1" := RVal_Bits [BV{32} 0] ]> $
-  <[ "EDSCR" := RVal_Bits [BV{32} 0] ]> $
-  <[ "MPIDR_EL1" := RVal_Bits [BV{64} 0] ]> $
   <[ "PSTATE" := (RegVal_Struct
     [("GE", RegVal_Poison); ("F", RegVal_Poison);
     ("UAO", RegVal_Poison); ("C", RVal_Bits [BV{1} 0]);
@@ -49,7 +38,18 @@ Definition sys_regs_map : reg_map :=
     ("IT", RegVal_Poison); ("IL", RegVal_Poison);
     ("Z", RVal_Bits [BV{1} 0]); ("BTYPE", RegVal_Poison);
     ("SSBS", RegVal_Poison); ("T", RegVal_Poison); ("J", RegVal_Poison);
-    ("V", RVal_Bits [BV{1} 0]); ("DIT", RegVal_Poison)]) ]> $ ∅.
+     ("V", RVal_Bits [BV{1} 0]); ("DIT", RegVal_Poison)]) ]> $
+  <[ "SCTLR_EL2" := RVal_Bits [BV{64} 0x0000000004000002] ]> $
+  <[ "SCR_EL3" := RVal_Bits [BV{32} 0] ]> $
+  <[ "TCR_EL2" := RVal_Bits [BV{64} 0] ]> $
+  <[ "CFG_ID_AA64PFR0_EL1_EL0" := RVal_Bits [BV{4} 1] ]> $
+  <[ "CFG_ID_AA64PFR0_EL1_EL1" := RVal_Bits [BV{4} 1] ]> $
+  <[ "CFG_ID_AA64PFR0_EL1_EL2" := RVal_Bits [BV{4} 1] ]> $
+  <[ "CFG_ID_AA64PFR0_EL1_EL3" := RVal_Bits [BV{4} 1] ]> $
+  <[ "OSLSR_EL1" := RVal_Bits [BV{32} 0] ]> $
+  <[ "OSDLR_EL1" := RVal_Bits [BV{32} 0] ]> $
+  <[ "EDSCR" := RVal_Bits [BV{32} 0] ]> $
+  <[ "MPIDR_EL1" := RVal_Bits [BV{64} 0] ]> $ ∅.
 
 Section sys_regs.
   Context `{!islaG Σ} `{!threadG}.
@@ -61,14 +61,12 @@ Section sys_regs.
     reg_col sys_regs ∗
     reg_col CNVZ_regs.
   Proof.
-    rewrite !reg_col_cons_Some !reg_col_cons_None reg_col_nil.
     repeat (rewrite big_sepM_insert;[ | by vm_compute]).
-    iIntros "Hctx H". repeat iDestruct "H" as "[$ H]".
-    iDestruct "H" as "[HPSTATE _]".
-    iMod (reg_mapsto_to_struct_reg_mapsto with "Hctx HPSTATE") as "[$ H]".
+    iIntros "Hctx [HPSTATE H]".
+    iMod (reg_mapsto_to_struct_reg_mapsto with "Hctx HPSTATE") as "[$ HPSTATE]".
     { simpl. repeat (constructor; [set_solver|]). constructor. }
-    simpl. iModIntro. iRevert "H".
-    repeat liAStep; liShow.
+    simpl. iModIntro. rewrite -(right_id True%I _ (reg_col CNVZ_regs)).
+    iRevert "H HPSTATE". repeat liAStep; liShow.
   Qed.
 End sys_regs.
 
